theories/parabstr/ws_deques_private.v
@@ -303,12 +303,13 @@ Section ws_deques_private_G.
   Proof.
   Admitted.
 
-  Lemma ws_deques_private_steal_to_spec t ι (sz : nat) i j :
+  Lemma ws_deques_private_steal_to_spec t ι (sz : nat) i i_ j :
     let j_ := Z.to_nat j in
-    (0 ≤ i < sz)%Z →
+    i = Z.of_nat i_ →
     (0 ≤ j < sz)%Z →
     <<<
-      ws_deques_private_inv t ι sz
+      ws_deques_private_inv t ι sz ∗
+      ws_deques_private_owner t i_
     | ∀∀ vss,
       ws_deques_private_model t vss
     >>>
@@ -324,7 +325,8 @@ Section ws_deques_private_G.
           ⌜vss !! j_ = Some (v :: vs)⌝ ∗
           ws_deques_private_model t (<[j_ := vs]> vss)
       end
-    | RET o; True
+    | RET o;
+      ws_deques_private_owner t i_
     >>>.
   Proof.
   Admitted.
