theories/parabstr/ws_deques_public.v
@@ -247,12 +247,13 @@ Section ws_deques_public_G.
         rewrite !list_insert_id //. iSteps.
   Qed.
 
-  Lemma ws_deques_public_steal_to_spec t ι (sz : nat) i j :
+  Lemma ws_deques_public_steal_to_spec t ι (sz : nat) i i_ j :
     let j_ := Z.to_nat j in
-    (0 ≤ i < sz)%Z →
+    i = Z.of_nat i_ →
     (0 ≤ j < sz)%Z →
     <<<
-      ws_deques_public_inv t ι sz
+      ws_deques_public_inv t ι sz ∗
+      ws_deques_public_owner t i_
     | ∀∀ vss,
       ws_deques_public_model t vss
     >>>
@@ -268,15 +269,16 @@ Section ws_deques_public_G.
           ⌜vss !! j_ = Some (v :: vs)⌝ ∗
           ws_deques_public_model t (<[j_ := vs]> vss)
       end
-    | RET o; True
+    | RET o;
+      ws_deques_public_owner t i_
     >>>.
   Proof.
-    iIntros "%j_ %Hi %Hj !> %Φ (%deques & %Hdeques_length & #Hdeques & #Hdeques_inv) HΦ".
+    iIntros (j_ -> Hj) "!> %Φ ((%deques & %Hdeques_length & #Hdeques & #Hdeques_inv) & Howner) HΦ".
     wp_rec.
     destruct (lookup_lt_is_Some_2 deques j_) as (deque & Hdeque_lookup); first lia.
     wp_smart_apply (array_unsafe_get_spec with "Hdeques") as "_"; [lia | done.. |].
     iDestruct (big_sepL_lookup with "Hdeques_inv") as "#Hdeque_inv"; first done.
-    awp_apply (inf_ws_deque_steal_spec with "Hdeque_inv").
+    awp_apply (inf_ws_deque_steal_spec with "Hdeque_inv") without "Howner".
     iApply (aacc_aupd_commit with "HΦ"); first done. iIntros "%vss (%_deques & _Hdeques & Hdeques_model)".
     iDestruct (array_model_agree with "Hdeques _Hdeques") as %<-. iClear "_Hdeques".
     iDestruct (big_sepL2_lookup_Some_l with "Hdeques_model") as %(vs & Hvss_lookup); first done.
